fv/lean/Ragu/Circuits/Element/Square.lean
@@ -3,6 +3,7 @@ import Ragu.Circuits.Element.Mul
 
 namespace Ragu.Circuits.Element.Square
 variable {p : ℕ} [Fact p.Prime]
+variable {ProverHint : Type}
 
 -- TODO: this is not necessary, there is `field`, but currently it's hard to
 -- work with, because Lean sometimes thinks `field T` and `T` are definitionally
@@ -11,7 +12,7 @@ structure Element (F : Type) where
   wire : F
 deriving ProvableStruct
 
-def main (input : Var Element (F p)) : Circuit (F p) (Var Element (F p)) := do
+def main (input : Var Element (F p)) : Circuit (F p) ProverHint (Var Element (F p)) := do
   let ⟨x⟩ := input
   return {
     wire := ←Mul.circuit ⟨x, x⟩
@@ -22,20 +23,20 @@ def Assumptions (_input : Element (F p)) := True
 def Spec (input : Element (F p)) (out : Element (F p)) :=
   out.wire = input.wire^2
 
-instance elaborated : ElaboratedCircuit (F p) Element Element where
+instance elaborated : ElaboratedCircuit (F p) ProverHint Element Element where
   main
   localLength _ := 3
 
-theorem soundness : Soundness (F p) elaborated Assumptions Spec := by
+theorem soundness : Soundness (F p) ProverHint elaborated Assumptions Spec := by
   circuit_proof_start
   simp [circuit_norm, Mul.circuit, Mul.Assumptions, Mul.Spec] at h_holds ⊢
   rw [h_holds]
   ring
 
-theorem completeness : Completeness (F p) elaborated Assumptions := by
+theorem completeness : Completeness (F p) ProverHint elaborated Assumptions := by
   circuit_proof_start [Mul.circuit, Mul.Assumptions]
 
-def circuit : FormalCircuit (F p) Element Element :=
+def circuit : FormalCircuit (F p) ProverHint Element Element :=
   { elaborated with Assumptions, Spec, soundness, completeness }
 
 end Ragu.Circuits.Element.Square
