fv/lean/Ragu/Instances/Autogen/Point/Double.lean
@@ -3,6 +3,8 @@ import Ragu.Core
 namespace Ragu.Instances.Autogen.Point.Double
 open Core.Primes
 
+variable {ProverHint : Type}
+
 @[reducible]
 def p := Core.Primes.p
 
@@ -13,20 +15,20 @@ def inputLen := 2
 def outputLen := 2
 
 set_option linter.unusedVariables false in
-def exportedOperations (input_var : Var (ProvableVector field inputLen) (F p)) : Operations (F p) := [
-  Operation.witness 3 (fun _env => default),
+def exportedOperations (input_var : Var (ProvableVector field inputLen) (F p)) : Operations (F p) ProverHint := [
+  Operation.witness 3 (fun _env _hint => default),
   Operation.assert ((((var 0) * (var 1)) + ((0x40000000000000000000000000000000224698fc094cf91b992d30ed00000000 : Expression (F p)) * (var 2)))),
   Operation.assert (((var 0) + ((0x40000000000000000000000000000000224698fc094cf91b992d30ed00000000 : Expression (F p)) * (input_var.get 0)))),
   Operation.assert (((var 1) + ((0x40000000000000000000000000000000224698fc094cf91b992d30ed00000000 : Expression (F p)) * (input_var.get 0)))),
-  Operation.witness 3 (fun _env => default),
+  Operation.witness 3 (fun _env _hint => default),
   Operation.assert ((((var 3) * (var 4)) + ((0x40000000000000000000000000000000224698fc094cf91b992d30ed00000000 : Expression (F p)) * (var 5)))),
   Operation.assert ((((0x0000000000000000000000000000000000000000000000000000000000000003 : Expression (F p)) * (var 2)) + ((0x40000000000000000000000000000000224698fc094cf91b992d30ed00000000 : Expression (F p)) * (var 5)))),
   Operation.assert ((((input_var.get 1) + (input_var.get 1)) + ((0x40000000000000000000000000000000224698fc094cf91b992d30ed00000000 : Expression (F p)) * (var 4)))),
-  Operation.witness 3 (fun _env => default),
+  Operation.witness 3 (fun _env _hint => default),
   Operation.assert ((((var 6) * (var 7)) + ((0x40000000000000000000000000000000224698fc094cf91b992d30ed00000000 : Expression (F p)) * (var 8)))),
   Operation.assert (((var 6) + ((0x40000000000000000000000000000000224698fc094cf91b992d30ed00000000 : Expression (F p)) * (var 3)))),
   Operation.assert (((var 7) + ((0x40000000000000000000000000000000224698fc094cf91b992d30ed00000000 : Expression (F p)) * (var 3)))),
-  Operation.witness 3 (fun _env => default),
+  Operation.witness 3 (fun _env _hint => default),
   Operation.assert ((((var 9) * (var 10)) + ((0x40000000000000000000000000000000224698fc094cf91b992d30ed00000000 : Expression (F p)) * (var 11)))),
   Operation.assert (((var 9) + ((0x40000000000000000000000000000000224698fc094cf91b992d30ed00000000 : Expression (F p)) * (var 3)))),
   Operation.assert (((var 10) + ((0x40000000000000000000000000000000224698fc094cf91b992d30ed00000000 : Expression (F p)) * ((input_var.get 0) + ((0x40000000000000000000000000000000224698fc094cf91b992d30ed00000000 : Expression (F p)) * ((var 8) + ((0x40000000000000000000000000000000224698fc094cf91b992d30ed00000000 : Expression (F p)) * ((input_var.get 0) + (input_var.get 0))))))))),
