fv/lean/Ragu/Instances/Autogen/Point/Negate.lean
@@ -3,6 +3,8 @@ import Ragu.Core
 namespace Ragu.Instances.Autogen.Point.Negate
 open Core.Primes
 
+variable {ProverHint : Type}
+
 @[reducible]
 def p := Core.Primes.p
 
@@ -13,7 +15,7 @@ def inputLen := 2
 def outputLen := 2
 
 set_option linter.unusedVariables false in
-def exportedOperations (input_var : Var (ProvableVector field inputLen) (F p)) : Operations (F p) := [
+def exportedOperations (input_var : Var (ProvableVector field inputLen) (F p)) : Operations (F p) ProverHint := [
 ]
 
 set_option linter.unusedVariables false in
