fv/lean/Ragu/Instances/Point/AddIncomplete.lean
@@ -24,6 +24,7 @@ def formal_instance : Core.Statements.GeneralFormalInstance where
   p
   inputLen
   outputLen
+  ProverHint := Circuits.Core.AllocMul.Row (F p)
   exportedOperations
   exportedOutput
 
@@ -63,7 +64,6 @@ def formal_instance : Core.Statements.GeneralFormalInstance where
 
   reimplementation :=
     Circuits.Point.AddIncomplete.circuit Circuits.Point.Spec.EpAffineParams
-      (Circuits.Core.AllocMul.readRow · 0)
 
   same_constraints := by
     intro input
