fv/lean/Ragu/Instances/Point/AllocFq.lean
@@ -18,6 +18,7 @@ def formal_instance : Core.Statements.GeneralFormalInstance where
   p
   inputLen
   outputLen
+  ProverHint := Circuits.Point.Alloc.Hint (F p)
   exportedOperations
   exportedOutput
 
@@ -30,8 +31,6 @@ def formal_instance : Core.Statements.GeneralFormalInstance where
   Spec input output := output.isOnCurve Circuits.Point.Spec.EqAffineParams
 
   reimplementation := Circuits.Point.Alloc.circuit Circuits.Point.Spec.EqAffineParams
-    (fun data => ((data "alloc_square_w" 1).getD 0 default)[0])
-    (fun data => ((data "alloc_square_w" 1).getD 2 default)[0])
 
   same_constraints := by
     intro input
